SeparationLogic/Upwards2Downwards.v
@@ -15,7 +15,7 @@ Local Open Scope KripkeSemantics.
 
 Module Upwards2Downwards.
 
-Definition dSM {L: Language} {nL: NormalLanguage L} {pL: PropositionalLanguage L} {SL: SeparationLanguage L} {MD: Model} {kMD: KripkeModel MD} (M: Kmodel) {kiM: KripkeIntuitionisticModel MD M} {SA: SeparationAlgebra MD M} {uSA: UpwardsClosedSeparationAlgebra MD M} {SM: Semantics L MD} {kiSM: KripkeIntuitionisticSemantics L MD M SM} {usSM: UpwardsSemantics L MD M SM}: @DownwardsSemantics.DownwardsSemantics L _ _ _ MD _ M kiM (DownwardsClosure_SA M) SM kiSM.
+Definition dsSM {L: Language} {nL: NormalLanguage L} {pL: PropositionalLanguage L} {SL: SeparationLanguage L} {MD: Model} {kMD: KripkeModel MD} (M: Kmodel) {kiM: KripkeIntuitionisticModel MD M} {SA: SeparationAlgebra MD M} {uSA: UpwardsClosedSeparationAlgebra MD M} {SM: Semantics L MD} {kiSM: KripkeIntuitionisticSemantics L MD M SM} {usSM: UpwardsSemantics L MD M SM}: @DownwardsSemantics.DownwardsSemantics L _ _ _ MD _ M kiM (DownwardsClosure_SA M) SM kiSM.
 Proof.
   constructor.
   + (* sat_sepcon *)
@@ -46,11 +46,19 @@ Proof.
         reflexivity.
 Defined.
 
+Definition UsSM {L: Language} {nL: NormalLanguage L} {pL: PropositionalLanguage L} {SL: SeparationLanguage L} {uSL: UnitarySeparationLanguage L} {MD: Model} {kMD: KripkeModel MD} (M: Kmodel) {kiM: KripkeIntuitionisticModel MD M} {SA: SeparationAlgebra MD M} {uSA: UpwardsClosedSeparationAlgebra MD M} {USA: UnitarySeparationAlgebra MD M} {nUSA: NormalUnitarySeparationAlgebra MD M} {SM: Semantics L MD} {kiSM: KripkeIntuitionisticSemantics L MD M SM} {usSM: UpwardsSemantics L MD M SM} {UsSM: UnitarySemantics L MD M SM} : @UnitarySemantics L _ _ _ _ MD _ M kiM (DownwardsClosure_SA M) (DownwardsClosure_USA M) SM kiSM.
+Proof.
+  constructor.
+  pose proof Korder_PreOrder as H_PreOrder.
+  intros; simpl.
+  apply sat_emp.
+Qed.
+
 End Upwards2Downwards.
 
 Module Upwards2Flat.
 
-Definition dSM {L: Language} {nL: NormalLanguage L} {pL: PropositionalLanguage L} {SL: SeparationLanguage L} {MD: Model} {kMD: KripkeModel MD} (M: Kmodel) {kiM: KripkeIntuitionisticModel MD M} {SA: SeparationAlgebra MD M} {uSA: UpwardsClosedSeparationAlgebra MD M} {SM: Semantics L MD} {kiSM: KripkeIntuitionisticSemantics L MD M SM} {usSM: UpwardsSemantics L MD M SM}: @FlatSemantics.FlatSemantics L _ _ _ MD _ M kiM (DownwardsClosure_SA M) SM kiSM.
+Definition fsSM {L: Language} {nL: NormalLanguage L} {pL: PropositionalLanguage L} {SL: SeparationLanguage L} {MD: Model} {kMD: KripkeModel MD} (M: Kmodel) {kiM: KripkeIntuitionisticModel MD M} {SA: SeparationAlgebra MD M} {uSA: UpwardsClosedSeparationAlgebra MD M} {SM: Semantics L MD} {kiSM: KripkeIntuitionisticSemantics L MD M SM} {usSM: UpwardsSemantics L MD M SM}: @FlatSemantics.FlatSemantics L _ _ _ MD _ M kiM (DownwardsClosure_SA M) SM kiSM.
 Proof.
   constructor.
   + (* sat_sepcon *)
@@ -77,5 +85,13 @@ Proof.
       exists m2; split; auto.
       reflexivity.
 Defined.
+
+Definition UsSM {L: Language} {nL: NormalLanguage L} {pL: PropositionalLanguage L} {SL: SeparationLanguage L} {uSL: UnitarySeparationLanguage L} {MD: Model} {kMD: KripkeModel MD} (M: Kmodel) {kiM: KripkeIntuitionisticModel MD M} {SA: SeparationAlgebra MD M} {uSA: UpwardsClosedSeparationAlgebra MD M} {USA: UnitarySeparationAlgebra MD M} {nUSA: NormalUnitarySeparationAlgebra MD M} {SM: Semantics L MD} {kiSM: KripkeIntuitionisticSemantics L MD M SM} {usSM: UpwardsSemantics L MD M SM} {UsSM: UnitarySemantics L MD M SM} : @UnitarySemantics L _ _ _ _ MD _ M kiM (DownwardsClosure_SA M) (DownwardsClosure_USA M) SM kiSM.
+Proof.
+  constructor.
+  pose proof Korder_PreOrder as H_PreOrder.
+  intros; simpl.
+  apply sat_emp.
+Qed.
 
 End Upwards2Flat.
